Use Fourier Transforms to solve $u_{xt} = 4u_x$, where $u(x, 0) = xe^{-x^2}$, with $x \in (-\infty, \infty)$ and $t \in [0, \infty)$

Here, let us take the fourier transform of both sides:
%
\begin{align}
  F[u_{xt}] & = i \xi \hat u_t\\
  F[4u_x] & = i \xi 4 \hat u
\end{align}

Here, both sides are equal to each other, so let us write:
%
\begin{align}
  i \xi \hat u_t & = i \xi 4 \hat u\\
  \hat u_t & = 4 \hat u
\end{align}

Here, let us find $u(x, t)$ by using our initial condition:
%
\begin{align}
  f(x) & = xe^{-x^2}
\end{align}

From here, let us consider the general solution for our function:
%
\begin{align}
  F[f(x)] & = \hat f(\xi)
\end{align}

Now, let us evaluate our fourier transform:
%
\begin{align}
  \hat u(\xi, t) & = A(\xi) e^{4t}
\end{align}

From here, let us evaluate at $t = 0$:
%
\begin{align}
  \hat u(\xi, 0) & = A(\xi) = \hat f(\xi)
\end{align}

So, let us write:
%
\begin{align}
  \hat u(\xi, t) & = \hat f(\xi) e^{4t}
\end{align}

From here, now that we have $\hat u$, let us retransform back:
%
\begin{align}
  u(x, t)
  & = \frac{1}{\sqrt{2 \pi}} \int^\infty_{-\infty} \hat f(\xi) e^{i \xi x} \text d \xi\\
  & = \frac{1}{\sqrt{2 \pi}} \int^\infty_{-\infty} \hat f(\xi)e^{4t} e^{i \xi x} \text d \xi\\
  & = \frac{e^{4t}}{\sqrt{2 \pi}} \int^\infty_{-\infty} \hat f(\xi) e^{i \xi x} \text d \xi\\
  & = e^{4t} f(x)
\end{align}
