\item Solve $u_{tt} = u_{xx}$ on $x \in [0, 1]$ if $u(0, t) = 5$, $u(1, t) = 2$, $u(x, 0) = x(1 - x) - 3x + 5$ and $u_t(x, 0) = 4$.

% Begin Answer
Here, let us write out our given conditions:
\begin{enumerate}
  \item $x \in [0, 1]$
  \item $u_{tt} = u_{xx}$
  \item $u\ (0, t) = 5$
  \item $u\ (1, t) = 2$
  \item $u\ (x, 0) = x(1 - x) - 3x + 5$
  \item $u_t(x, 0) = 4$
\end{enumerate}

Here, similar to the last problem, let us consider $w$ through $T_1$ and $T_1$:
%
\begin{align}
  \frac{T_1 - T_2}{L} & = (2 - 5)x + 2\\
  & = 3x - 5
\end{align}

Now, let us consider our steady state:
%
\begin{align}
  u(0, t) & = 5 \Rightarrow w(0, t) = u(0, t) - u(0, \infty) = 5 - 5 = 0\\
  u(0, t) & = 5 \Rightarrow w(0, t) = u(0, t) - u(0, \infty) = 2 - 2 = 0
\end{align}

Now, let us begin:
%
\begin{enumerate}
  \item Let us assume $w(x, t) = X(x)T(t)$
  %
  \begin{align}
    XT^{\prime\prime} & = X^{\prime\prime}T\\
    \frac{T^{\prime\prime}}{T} & = \frac{X^{\prime\prime}}{X} = - \lambda
  \end{align}

  \item Let us solve for $X$
  %
  \begin{align}
    X^{\prime\prime} & = - \lambda X
  \end{align}

  Here, let us use the general cosine, sine form:
  %
  \begin{align}
    X(x) & = A \sin \left(\sqrt \lambda x \right) + B \cos \left(\sqrt \lambda x \right)\\
    X(0) = 0 & = B\\
    X(x) & = A \sin \left( \sqrt \lambda x \right)\\
    X(1) = 0 & = A \sin \left( \sqrt \lambda 1 \right)\\
    n \pi & = \sqrt \lambda 1\\
    \sqrt \lambda & = n \pi\\
    \lambda_n & = (n \pi)^2\\
    X_n(x) & = \sin(n \pi x)
  \end{align}

  \item Let us solve for $T_n$
  %
  \begin{align}
    T^{\prime\prime}_n(t) & = - (n \pi)^2T\\
    T_n(t) & = C_n \cos(n \pi t) + D_n \sin(n \pi t)
  \end{align}

  \item Combine and find $w_n$ and $w$

  Here, let us combined our values:
  %
  \begin{align}
    w_n(x, t) & = \sin(n \pi x)\left[ C_n \cos(n \pi t) + D_n \sin(n \pi t) \right]
  \end{align}

  By linearity,
  %
  \begin{align}
    w(x, t) & = \sum^\infty_{n = 1}
    \sin(n \pi x)\left[ C_n \cos(n \pi t) + D_n \sin(n \pi t) \right]\\
    & = \sum^\infty_{n = 1}
    C_n \sin(n \pi x) \cos(n \pi t) + D_n \sin(n \pi x) \sin(n \pi t)
  \end{align}

  \item Let us find the coefficients using the initial condition:
  %
  \begin{align}
    w(x, t) & = \sum^\infty_{n = 1}
    C_n \sin(n \pi x) \cos(n \pi t) + D_n \sin(n \pi x) \sin(n \pi t)\\
    w_t(x, t) & = \sum^\infty_{n = 1}
    -C_n n \pi \sin(n \pi x) \sin(n \pi t) + D_n n \pi \sin(n \pi x) \cos(n \pi t)\\
    w_t(x, 0) & = \sum^\infty_{n = 1}
    D_n n \pi \sin(n \pi x) = 4
  \end{align}

  Here, let us integrate:
  %
  \begin{align}
    D_n n \pi & = 2 \int^1_0 4 \sin(n \pi x) \text{ dx}\\
    D_n & = \frac{8}{n \pi} \int^1_0 \sin(n \pi x) \text{ dx}\\
    & = - \frac{8}{n \pi} \frac{1}{n \pi} \cos(n \pi x) \Big|^1_0\\
    & = - \frac{8}{n^2 \pi^2} \cos(n \pi x) \Big|^1_0\\
    & = - \frac{8}{n^2 \pi^2} (\cos(n \pi) - 1)\\
    & = \frac{8}{n^2 \pi^2} (1 - \cos(n \pi))\\
    & \Rightarrow \frac{8}{n^2 \pi^2} (1 - (-1)^n)
  \end{align}

  Now, let us find $w(x, 0)$:
  %
  \begin{align}
    w(x, t) & = \sum^\infty_{n = 1} C_n \sin(n \pi x) \cos(n \pi t) + \frac{8}{n^2 \pi^2} (1 - (-1)^n) \sin(n \pi x) \sin(n \pi t)\\
    w(x, 0) & = \sum^\infty_{n = 1} C_n \sin(n \pi x) = x - x^2
  \end{align}

  Here, let us integrate:
  %
  \begin{align}
    C_n & = 2 \int^1_0 x \sin(n \pi x) - x^2 \sin(n \pi x)
  \end{align}
\end{enumerate}

Let us create our integration tables:
%
\begin{center}
  \begin{tabular}{c|c}
    $x$ & $\sin(n \pi x)$\\
    \hline
    $1$ & $-\frac{1}{n \pi} \cos(n \pi x)$\\
    \hline
    $0$ & $-\frac{1}{n^2 \pi^2} \sin(n \pi x)$\\
    &
  \end{tabular}
  \begin{tabular}{c|c}
    $x^2$ & $\sin(n \pi x)$\\
    \hline
    $2x$ & $-\frac{1}{n \pi} \cos(n \pi x)$\\
    \hline
    $2$ & $-\frac{1}{n^2 \pi^2} \sin(n \pi x)$\\
    \hline
    $0$ & $\frac{1}{n^3 \pi^3} \cos(n \pi x)$
  \end{tabular}
\end{center}

Here, we have:
%
\begin{align}
  C_n & = 2 \left(
  \frac{x}{n \pi} \cos(n \pi x) - \frac{1}{n^2 \pi^2} \sin(n \pi x) -
  \frac{x^2}{n \pi} \cos(n \pi x) + \frac{2x}{n^2 \pi^2} \sin(n \pi x) + \frac{2}{n^3 \pi^3} \cos(n \pi x)
  \right)^1_0\\
  & = 2 \left( \frac{1}{n \pi} \cos(n \pi) - \frac{1}{n \pi} \cos(n \pi) - \frac{2}{n^3 \pi^3} \cos(n \pi) + \frac{2}{n^3 \pi^3} \right)\\
  & = 2 \left( - \frac{2}{n^3 \pi^3} \cos(n \pi) + \frac{2}{n^3 \pi^3} \right)\\
  & = 4 \left(\frac{1 - \cos(n \pi)}{n^3 \pi^3} \right)\\
  & = \left(\frac{4 - 4\cos(n \pi)}{n^3 \pi^3} \right)
\end{align}

Now, our heat equation is:
%
\begin{align}
  u(x, t) & =
  \sum^\infty_{n = 1} \frac{4 - 4\cos(n \pi)}{n^3 \pi^3} \sin(n \pi x) \cos(n \pi t) + \frac{8}{n^2 \pi^2} (1 - (-1)^n) \sin(n \pi x) \sin(n \pi t) - 3x + 5
\end{align}
