\item Show that the convolution of two functions can be written as either:
%
\begin{align*}
  (f * g) (x) & = \frac{1}{\sqrt{2 \pi}} \int^\infty_{-\infty} f(x - \xi) g(\xi) \text{ d}\xi
\end{align*}

or
%
\begin{align*}
  (f * g) (x) & = \frac{1}{\sqrt{2 \pi}} \int^\infty_{-\infty} f(\xi) g(x - \xi) \text{ d}\xi
\end{align*}

In other words, show they are equivalent.

% Need this in the heat equation
% Use convolution

\begin{proof}
  Here, let us prove both equations are equivalent,

Here, let us work with the first equation to get to the second equation.

Here, let us consider our function:
%
\begin{align}
  (f * g)(x) & = \frac{1}{\sqrt{2 \pi}} \int^\infty_{-\infty} f(x - \xi) g(\xi) \text{ d}\xi
\end{align}

Here, let us consider substituting the inside of our equation with the following:
%
\begin{align}
  u & = x - \xi\\
  \text du & = - \text d\xi\\
  - \text du & = \text d\xi
\end{align}

Here, instead of using $u$, let us use $x - u$.

Furthermore, let us consider our domain of integration and input them into $u$:
%
\begin{align}
  u(x) & = x - \xi\\
  u(\infty) & = x - \infty\\
  & = -\infty\\
  u(-\infty) & = x - - \infty\\
  & = x + \infty\\
  & = \infty
\end{align}

Now, let us execute the substitution in our first equation:
%
\begin{align}
  (f * g)(x)
  & =
  \frac{1}{\sqrt{2 \pi}}
  \int^\infty_{-\infty}
  f(x - \xi) g(\xi) \text d \xi\\
  & =
  -\frac{1}{\sqrt{2 \pi}}
  \int^{-\infty}_\infty
  f(u) g(x - u) \text du
\end{align}

Here, let us flip our integral,
%
\begin{align}
  & =
  -\frac{1}{\sqrt{2 \pi}}
  \int^{-\infty}_\infty
  f(u) g(x - u) \text du\\
  (f * g)(x) & =
  \frac{1}{\sqrt{2 \pi}}
  \int^{\infty}_{-\infty}
  f(u) g(x - u) \text du
\end{align}
% u sub in problem

Here, using $u$ substitution, we have reached the second given equation by using the first equation. The convolution of the two functions are equivalent.

\end{proof}
