\item Solve the following equations using the method of characteristics
\begin{enumerate}
  \item $u_t + 7u_x = t$ \quad $u(x, 0) = \sin x$
  \item $u_t + xu_x + 2u = 0$ \quad $u(x, 0) = x^3$
  \item $u_t + 2xtu_x = u$ \quad $u(x, 0) = 1 - x$
  \item $tu_t + 2xu_x = t\sin(\pi t)$ \quad $u(x, 1) = \cos x$
\end{enumerate}
\bigbreak
%____________________________________________________________________________%

\begin{enumerate}
  \item Part a
  \item Here, let us consider rewriting our equation:
  %
  \begin{align}
    u_t + xu_x & = -2u
  \end{align}

  From here, we can find:
  %
  \begin{align}
    \frac{dx}{ds} & = x\\
    \frac{dt}{ds} & = 1\\
    \frac{du}{ds} & = -2u
  \end{align}

  Here, finding $\frac{dx}{ds}$ is a matter of solving a differential equation to get:
  %
  \begin{align}
    \frac{dx}{ds} & = x\\
    x & = ce^s
  \end{align}

  Next, we can also find our second term for $\frac{dt}{ds}$ and find:
  %
  \begin{align}
    \frac{dt}{ds} & = 1\\
    dt & = ds\\
    t & = s + t_0 = s
  \end{align}

  Note since $s = t$, we can replace this for what we found with $x$.
  Now, to find
  $\frac{dt}{ds}$,
  let us take a similar approach as with
  $\frac{dx}{ds}$ and write:
  %
  \begin{align}
    \frac{du}{ds} & = -2u\\
    u & = de^{-2s}
  \end{align}

  Here, recall $s = t$. We also are given $u(0)$ as $x^3$:
  %
  \begin{align}
    u & = de^{-2s}\\
    u & = u_0 e^{-2t}\\
    u & = f\left( x_0 \right) e^{-2t}
  \end{align}

  From here, let us take a look back at $x$ and find $x_0$:
  %
  \begin{align}
    x & = ce^t\\
    x & = x_0 e^t\\
    x e^{-t} & = x_0
  \end{align}

  Now, if we plug $x_0$ into $u$, we can find:
  %
  \begin{align}
    u & = f\left( x_0 \right) e^{-2t}\\
    u & = f\left( x e^{-t} \right) e^{-2t}\\
    u & = \left(x e^{-t}\right)^3 e^{-2t}\\
    u & = x^3 e^{-3t} e^{-2t}\\
    u & = x^3 e^{-5t}
  \end{align}

  \item Here, let us rewrite our equation:
  %
  \begin{align}
    u_t + 2x tu_x & = u\\
    u(x, 0) & = 1 - x
  \end{align}

  Here, note that $u_x$ has $t$ as a coefficient. Let us skip over the change of variable ($t = s$) and write:
  %
  \begin{align}
    \frac{dx}{dt} & = 2xt\\
    \frac{du}{dt} & = u
  \end{align}

  First, let us consider solving for $\frac{dx}{dt}$.
  Here, let us solve the differential equation:
  %
  \begin{align}
    \frac{dx}{dt} & = 2xt\\
    \int \frac{1}{x}\ dx & = \int 2t\ dt\\
    \ln |x| & = t^2 + c\\
    x & = ce^{t^2}\\
    x & = x_0 e^{t^2}
  \end{align}

  Now, let us solve for $\frac{du}{dt}$:
  %
  \begin{align}

  \end{align}
\end{enumerate}
