\subsection*{March 4, 2022}

\topic{Wave Equation}

Here, let us consider the following conditions:
%
\begin{itemize}
  \item $u_{tt} = u_{xx}$, $t \in [0, \infty), x \in (-\infty, \infty)$
  \item $\displaystyle \lim_{x \to \pm \infty} u(x, t) = 0$
  \item $u(x, 0) = f(x)$
  \item $u_t(x, 0) = g(x)$
\end{itemize}

\note Two initial conditions for wave: Heat's condition $(u(x, 0) = f(x))$ and $u_t(x, 0) = g(x)$

Now, let us begin:
%
\begin{enumerate}
  \item Let us solve $F$:
  %
  \begin{align}
    F[u_{tt}] & = F[u_{xx}]\\
    \Rightarrow \hat u_{tt} & = (i \xi)^2 \hat u\\
    \Rightarrow \hat u_{tt} & = - \xi^2 \hat u\\
    \hat u(\xi, 0) & = \hat f(\xi)
  \end{align}

  Now, let us consider $\hat u_t(\xi, 0)$:
  %
  \begin{align}
    F[u_t(x, 0)] & = \frac{1}{\sqrt{2 \pi}} \int^\infty_{-\infty} u_t(x, 0) e^{-i x \xi} \text{ dx}\\
    & = \frac{1}{\sqrt{2 \pi}} \int^\infty_{-\infty} g(x) e^{-i x \xi} \text{ dx}\\
    & = \hat g(\xi)
  \end{align}

  \item Solve $\hat u_{tt} = -\xi^2 \hat u$ with the following conditions:
  \begin{itemize}
    \item $\hat u(\xi, 0) = \hat f(\xi)$
    \item $\hat u_t(\xi, 0) = \hat g(\xi)$
  \end{itemize}

  Now let us write the general form:
  %
  \begin{align}
    \hat u(\xi, t) & = A(\xi) \sin(\xi t) + B(\xi) \cos(\xi t)
  \end{align}

  Here, we do not want to use sine and cosine because we will multiply by expontentials later on.
  %
  \begin{align}
    \hat u(\xi, t) & = A(\xi) e^{i \xi t} + B(\xi) e^{-i \xi t}\\
    \hat u(\xi, 0) & = A(\xi) + B(\xi) = \hat f(\xi)
  \end{align}

  Here, let us find the $t$ partial,
  %
  \begin{align}
    \hat u_t(\xi, t) & = i \xi A(\xi) e^{i \xi t} - i \xi B(\xi) e^{- i \xi t}\\
    \hat u (\xi, 0) & = i \xi A(\xi) - i \xi B(\xi) = \hat g(\xi)
  \end{align}

  Here, let us take the equation with $\hat f(\xi)$ and multiply it by $i \xi$:
  %
  \begin{align}
    2 i \xi A(\xi) & = i \xi \hat f(\xi) + \hat g (\xi)\\
    a(\xi) & = \frac{\hat f(\xi)}{2} + \frac{\hat g(\xi)}{2 i \xi}
  \end{align}

  Now, let us subtract to find $B$:
  %
  \begin{align}
    2 i \xi B(\xi) & = i \xi \hat f (\xi) - \hat g (\xi)\\
    B(\xi) & = \frac{\hat f(\xi)}{2} - \frac{\hat g(\xi)}{2 i \xi}
  \end{align}

  Here, substitute in our terms:
  %
  \begin{align}
    \hat u(\xi, t)
    & = \left[ \frac{\hat f(\xi)}{2} + \frac{\hat g(\xi)}{2 i \xi}  \right] e^{i \xi t} + \left[ \frac{\hat f(\xi)}{2} - \frac{\hat g(\xi)}{2 i \xi} \right] e^{-i \xi t}
  \end{align}

  \item Retransform
  %
  \begin{align}
    u(x, t)
    & = \frac{1}{\sqrt{2 \pi}} \int^\infty_{-\infty} \hat u(\xi, t) e^{i x \xi} \text{ d}\xi\\
    & = \frac{1}{\sqrt{2 \pi}} \int^\infty_{-\infty} \left[ \frac{\hat f(\xi)}{2} + \frac{\hat g(\xi)}{2 i \xi}  \right] e^{i \xi t} + \left[ \frac{\hat f(\xi)}{2} - \frac{\hat g(\xi)}{2 i \xi} \right] e^{-i \xi t} \text{ d}\xi\\
    & =
    \frac{1}{2 \sqrt{2 \pi}} \int^\infty_{-\infty}
    \hat f(\xi)
    \left(e^{i \xi t} + e^{-i \xi t}\right)e^{i x \xi} +
    \frac{\hat g(\xi)}{i \xi}
    \left( e^{i \xi t} - e^{-i \xi t} \right)e^{i x \xi} \text{ d}\xi\\
    & =
    \frac{1}{2 \sqrt{2 \pi}} \int^\infty_{-\infty}
    \hat f(\xi) \left[ e^{i \xi(x + t)} + e^{i \xi(x - t)} \right] \text{ d}\xi
    + \frac{1}{2 \sqrt{2 \pi}} \int^\infty_{-\infty}
    \frac{\hat g(\xi)}{i \xi}
    \left[ e^{i \xi(x + t)} - e^{i \xi(x - t)} \right] \text{ d}\xi
  \end{align}

  We know that
  %
  \begin{align}
    f(x) & = \frac{1}{\sqrt{2 \pi}} \int^\infty_{-\infty} \hat f(\xi) e^{i x \xi} \text{ d}\xi\\
    f(x + t) & = \frac{1}{\sqrt{2 \pi}} \int^\infty_{-\infty} \hat f(\xi) e^{i \xi(x + t)} \text{ d}\xi\\
    f(x - t) & = \frac{1}{\sqrt{2 \pi}} \int^\infty_{-\infty} \hat f(\xi) e^{i \xi(x - t)} \text{ d}\xi
  \end{align}

  From the previous two equations, let us write:
  %
  \begin{align}
    \frac{1}{2} \left[ f(x + t) + f(x - t) \right]\\
    & = \frac{1}{2} \left[ f(x + t) + f(x - t) \right] +
    \frac{1}{2 \sqrt{2 \pi}} \int^\infty_{-\infty} \frac{\hat g(\xi)}{i \xi} \left( e^{i \xi(x + t)} - e^{i \xi(x - t)} \right) \text{ d}\xi
  \end{align}

  Now, let us write:
  %
  \begin{align}
    \frac{\hat g(\xi)}{i \xi}
    & = \frac{\frac{1}{\sqrt{2\pi}} \int^\infty_{-\infty} g(x)e^{-i x \xi} \text{ dx}}{i \xi}\\
    & = \frac{1}{\sqrt{2 \pi}} \int^\infty_{-\infty} \frac{g(x)e^{-i x \xi} }{i \xi} \text{ dx}
  \end{align}

  Here, we consider integral by parts: $u = \frac{e^{- x \xi}}{- i \xi} \Rightarrow du = e^{- i \xi} \text{ dx}$ and $dv = g(x) \text{ dx} \Rightarrow v = \int^x_{-\infty} g(y) \text{ dy}$.
  %
  \begin{align}
    & = - \frac{1}{\sqrt{2 \pi}}
    \left[
    \int^x_{-\infty} g(y) \text{ dy } \frac{e^{-i \xi x}}{- i \xi} \Big|^\infty_{-\infty} - \int^\infty_{-\infty} \int^x_{-\infty} g(y) \text{ dy } e^{-i x \xi} \text{ dx}
    \right]\\
    & = \hat h(\xi)
  \end{align}

  Now, from the two equations, let us consider $f(x - t)$:
  %
  \begin{align}
    & = \frac{1}{2} \left[ f(x + t) + f(x - t) \right] + \frac{1}{2 \sqrt{2 \pi}} \int^\infty_{-\infty} \hat h(\xi) \left( e^{i \xi(x + t)} - e^{i \xi(x - t)} \right)\ text{ d}\xi\\
    & = \frac{1}{2} \left[ f(x + t) + f(x - t) \right] + \frac{1}{2} \left[ h(x + t) - h(x - t)\right]\\
    & = \frac{1}{2} \left[ f(x + t) + f(x - t) \right]
    + \frac{1}{2} \left[ \int^{x + t}_{- \infty} g(y) \text{ dy } - \int^{x - t}_{-\infty} g(y) \text{ dy} \right]\\
    & = \frac{1}{2} \left[ f(x + t) + f(x - t) \right]
    + \frac{1}{2} \int^{x + t}_{x - t} g(y) \text{ dy}
  \end{align}

  This is the solution to the wave equation on an infinite domain called D'Alembert's Formula.
  %
\end{enumerate}

\hrulefill
